spec/design/ArchVSpaceDecls_H.thy
@@ -225,7 +225,7 @@ consts
 checkVPAlignment :: "vmpage_size \<Rightarrow> vptr \<Rightarrow> ( syscall_error , unit ) kernel_f"
 
 consts
-validMappingSize :: "vmpage_size \<Rightarrow> kernel_state \<Rightarrow> bool"
+checkValidMappingSize :: "vmpage_size \<Rightarrow> unit kernel"
 
 consts
 performARMMMUInvocation :: "ArchRetypeDecls_H.invocation \<Rightarrow> machine_word list kernel_p"
