spec/design/Structures_H.thy
@@ -1968,4 +1968,5 @@ defs maxFreeIndex_def:
 "maxFreeIndex magnitudeBits \<equiv> bit magnitudeBits"
 
 
+
 end
